chore: bump lean4 dep to leanprover/lean4:nightly-2021-08-18

deps/galois_stdlib/src/Galois/Data/RBMap.lean
@@ -3,34 +3,34 @@ import Std.Data.RBMap
 
 namespace Std
 namespace RBMap
-universes u v w
+universe u v w
 variable {α : Type u} {β : Type v}
 
 /- Builds an RBMap from a list with String keys. -/
-def ltMap [HasLess α] [∀ (a b : α), Decidable (a < b)] (entries: List (α × β))
- : RBMap α β (λ (x y:α)=> x<y) :=
- RBMap.fromList entries (λ (x y:α)=> x<y)
+def ordMap [Ord α] (entries: List (α × β))
+ : RBMap α β Ord.compare :=
+ RBMap.fromList entries Ord.compare
 
 
 section
-variable {lt : α → α → Bool}
+variable {cmp : α → α → Ordering}
 
-@[specialize] def keys : RBMap α β lt → List α
+@[specialize] def keys : RBMap α β cmp → List α
   | ⟨t, _⟩ => t.revFold (fun ps k _v => k::ps) []
 
-@[specialize] def values : RBMap α β lt → List β
+@[specialize] def values : RBMap α β cmp → List β
   | ⟨t, _⟩ => t.revFold (fun ps _k v => v::ps) []
 
-@[inline] def map {σ : Type w} (f : α → β → σ) : RBMap α β lt → RBMap α σ lt
+@[inline] def map {σ : Type w} (f : α → β → σ) : RBMap α β cmp → RBMap α σ cmp
   | ⟨t, _⟩ => t.fold (λ acc k v => acc.insert k (f k v)) RBMap.empty
 
 /- Appends two RBMaps, with the second argument's entries overwriting
     any entries in the first argument where applicable. -/
-@[specialize] def append (lhs rhs : RBMap α β lt) : RBMap α β lt :=
+@[specialize] def append (lhs rhs : RBMap α β cmp) : RBMap α β cmp :=
   if lhs.isEmpty then rhs
   else rhs.fold (λ m k v => m.insert k v) lhs
 
-instance : Append (RBMap α β lt) := ⟨RBMap.append⟩
+instance : Append (RBMap α β cmp) := ⟨RBMap.append⟩
 
 end
 
@@ -39,7 +39,7 @@ end RBMap
 namespace RBMap
 
 -- It's not happy about the universes on this one if we try and add the level parameters (and even use max/ULift/etc) =\
-@[inline] def mapM {α β σ : Type} {lt : α → α → Bool} {m : Type → Type} [Monad m] (f : α → β → m σ) : RBMap α β lt → m (RBMap α σ lt)
+@[inline] def mapM {α β σ : Type} {cmp : α → α → Ordering} {m : Type → Type} [Monad m] (f : α → β → m σ) : RBMap α β cmp → m (RBMap α σ cmp)
   | ⟨t, _⟩ => t.foldM (λ acc k v => acc.insert k <$> (f k v)) RBMap.empty
 
 
